snapshot.thy
@@ -18,6 +18,9 @@ abbreviation "snapshot_num s e \<equiv> case (snapshot_map s).[e] of Some n \<Ri
 definition includedIn where
 "includedIn e n snapshot \<equiv> n < snapshot_num snapshot e"
 
+definition includedIn' (infixl "\<in>\<^sub>s" 40) where
+"e \<in>\<^sub>s snapshot \<equiv> snd e < snapshot_num snapshot (fst e)"
+
 find_consts "'k \<Rightarrow> 'v \<Rightarrow> ('k,'v) fmap \<Rightarrow> ('k,'v) fmap"
 
 definition snapshot_update  :: "snapshot \<Rightarrow> event \<Rightarrow> nat \<Rightarrow> snapshot" where
